LeanBoogie/Boogie.lean
@@ -1,0 +1,85 @@
+import Std
+import Aesop
+import LeanBoogie.ITree
+import LeanBoogie.Notation
+import LeanBoogie.Iter
+
+namespace LeanBoogie
+
+open Std (HashSet HashMap)
+
+/-
+  # Boogie state monad
+  Tracks values of boogie variables during execution.
+-/
+
+
+/-- Assigns values to every variable. Ideally you'd want `(v : String) -> v ∈ ValidVars -> Int`. -/
+abbrev BoogieState := String -> Int
+
+def BoogieState.update (v : String) (val : Int) : BoogieState -> BoogieState :=
+  fun σ v' => if _h : v' = v then val else σ v'
+instance : EmptyCollection BoogieState := ⟨fun _ => 0⟩
+
+
+/-- State monad during execution of boogie programs. Assigns values to every variable. -/
+abbrev Boogie (E : Type) : Type -> Type := StateT BoogieState (ITree E)
+
+def Boogie.read (v : String) : Boogie E Int := fun σ => pure (σ v, σ)
+def Boogie.write (v : String) (val : Int) : Boogie E Unit := fun σ => pure ((), BoogieState.update v val σ)
+/-- Apply a pure function to a variable. Useful for simple operations such as increments, setting to zero, etc. -/
+def Boogie.update (v : String) (f : Int -> Int) : Boogie E Unit
+  := Boogie.read v >>= fun x => Boogie.write v (f x)
+
+
+/- ## Helpers for writing imperative programs.  -/
+
+def Boogie.iter (f : A -> Boogie E (A ⊕ B)) : A -> Boogie E B := sorry
+instance : Iter (Boogie E) := ⟨Boogie.iter⟩
+
+def Boogie.skip : Boogie E Unit := pure ()
+def Boogie.seq (a b : Boogie E Unit) : Boogie E Unit := a >>= (fun () => b)
+instance : Seqi (Boogie E Unit) := ⟨Boogie.seq⟩
+
+def Boogie.case (t e : Boogie E A) : Bool -> Boogie E A
+| true => t
+| false => e
+
+def Boogie.ite (c : Boogie E Bool) (t e : Boogie E A) : Boogie E A :=
+  c >>= Boogie.case t e
+
+abbrev Boogie.pure : A -> Boogie E A := Pure.pure
+abbrev Boogie.bind : (Boogie E A) -> (A -> Boogie E B) -> Boogie E B := Bind.bind
+
+/-- Actually execute a boogie program, starting with every variable being 0-initialized. -/
+def Boogie.run (m : Boogie Empty Unit) (fuel : Nat) : Option BoogieState :=
+  let s₀ : BoogieState := (fun _ => 0)
+  let stuff := StateT.run m s₀
+  let ⟨_, ret⟩ := ITree.run stuff Empty.elim fuel
+  ret.map Prod.snd
+
+/-- Equivalence up-to-tau, but adapted for the `Boogie` monad. -/
+def EuttB (b1 : Boogie E A) (b2 : Boogie E A) : Prop := ∀σ : BoogieState, Eutt (b1 σ) (b2 σ)
+infixr:20 " ~=~ " => EuttB
+
+axiom EuttB.eq {E A : Type} {x y : Boogie E A} : EuttB x y -> x = y
+
+theorem Boogie.ite_push_state [Decidable c] {t e : Boogie E A}
+  : (if c then t else e) σ ~~ (if c then t σ else e σ)
+  := by split; repeat exact Eutt.refl _
+
+theorem Boogie.bind_push_state {a : Boogie E A} {b : A -> Boogie E B}
+  : (a >>= b) σ ~~ (a σ >>= fun res => b res.fst res.snd)
+  := sorry
+
+def Boogie.while_ (c : Boogie E Bool) (body : Boogie E Unit) : Boogie E Unit :=
+  Boogie.iter
+    (fun () => Boogie.ite c
+      (do body; return .inl ())
+      (return .inr ()))
+    ()
+
+@[simp] theorem ite_bind [Monad m] [Decidable c] {m1 m2 : m a} {k : a -> m b}
+  : (if c then m1       else m2      ) >>= k
+  =  if c then m1 >>= k else m2 >>= k
+  := by aesop
