LeanBoogie/ITree/ITree0W.lean
@@ -1,0 +1,98 @@
+import LeanBoogie.ITree.ITree
+import LeanBoogie.ITree.Eutt
+import LeanBoogie.Notation
+import LeanBoogie.ITree.KTree -- just for fmap, inr
+
+namespace LeanBoogie
+open ITree
+
+-- # ITree Specs Without Effects [DM4Ever]
+-- See section 4 of "Dijkstra Monads for ever".
+
+-- Corresponding computation monad: `ITree Empty`.
+abbrev ITree0 (A : Type) := ITree Empty A
+def Converges (a : A) (t : ITree0 A) : Prop := t ~~ .ret a
+def Diverges (t : ITree0 A) : Prop := t ~~ spin
+
+/-- The predicate `P` respects equivalence up to tau. -/
+def RespEutt (P : ITree0 A -> Prop) : Prop := ∀t1 t2 : ITree0 A, Eutt t1 t2 -> P t1 -> P t2
+
+/-- Source: https://lag47.github.io/assets/pdf/dissertation.pdf definition 9,
+  and the Interaction Trees repo `PureITreeDijkstra.v` definition `monotonici`.  -/
+def Monotonic (w : (p : ITree0 A -> Prop) -> (_ : RespEutt p) -> Prop) : Prop :=
+  (p1 p2 : ITree0 A -> Prop) -> {h1 : RespEutt p1} -> {h2 : RespEutt p2} ->
+      (∀t : ITree0 A, p1 t -> p2 t) ->
+        @w p1 h1 ->
+        @w p2 h2
+
+/-- Specification monad for eventless interaction trees. In the Dijkstra Monads for ever paper,
+  this is called `DelaySpec`. We require the specification to adhere to some properties (mono, respeutt)
+  but that is not very relevant for generating verification conditions.
+  You should be able to pretend this is just `def ITree0W (A) := (ITree0 A -> Prop) -> Prop`. -/
+def ITree0W (A : Type) := (w : (p : ITree0 A -> Prop) -> (_ : RespEutt p) -> Prop) ×' Monotonic w
+
+def ITree0W.pure {A   : Type} (a : A) : ITree0W A := ⟨
+  fun (post : ITree Empty A -> Prop) _ => post (Pure.pure a),
+  fun p1 p2 h1 _ t h => by simp_all only⟩
+
+def ITree0W.bind {A B : Type} (wa : ITree0W A) (wb : A -> ITree0W B) : ITree0W B := ⟨
+  fun (post : ITree Empty B -> Prop) hpost =>
+    wa.1 (fun ta => (∃a:A, Converges a ta ∧ (wb a).1 post hpost) ∨ Diverges ta) (by sorry),
+  by
+    unfold Converges Diverges
+    intro p1 p2 p1h p2h t h
+    unfold ITree0W at wa wb
+    obtain ⟨wa, wah⟩ := wa
+    -- obtain ⟨wb, wbh⟩ := wb ?a
+    simp only at *
+    sorry
+⟩
+
+instance : Monad ITree0W where
+  pure := .pure
+  bind := .bind
+instance : LawfulMonad ITree0W := sorry
+
+
+-- ## Morphism θ from ITree0 to ITree0W
+
+def ITree0.θ (t : ITree0 A) : ITree0W A := ⟨fun post _hpost => post t, by intro _ _ _ _ _ _; simp_all only⟩
+instance : Theta ITree0 ITree0W := ⟨ITree0.θ⟩
+
+def ITree0W.le (w1 w2 : ITree0W A) : Prop := ∀p, (hp : RespEutt p) -> w2.1 p hp -> w1.1 p hp
+instance : LE (ITree0W A) := ⟨ITree0W.le⟩
+
+theorem ITree0.θ_pure : θ (return a) = return a := rfl
+theorem ITree0.θ_bind {a : ITree0 A} {b : A -> ITree0 B}
+  : θ (a >>= b) = (θ a >>= fun a => θ (b a))
+  := by
+    dsimp [Bind.bind, ITree.bind, ITree0W.bind]
+    -- ! This will be a substantial chunk of work, because you need to dig into coinduction
+    sorry
+
+instance : LawfulTheta ITree0 ITree0W := ⟨ITree0.θ_pure, ITree0.θ_bind⟩
+
+theorem θ_if {t e : ITree0 A} [Decidable c] : θ (if c then t else e) = if c then θ t else θ e := by
+  sorry
+
+
+-- ## Specs for Iter
+
+-- /-- From the Interaction Trees repo, `PureITreeDijkstra.v` definition `iterp`.
+--   This is a convoluted coinductive definition in the Coq repo. -/
+-- def ITree0W.iter (f : A -> ITree0W (A ⊕ B)) (a : A) : ITree0W B := ⟨
+--   fun post hpost => sorry,
+--   sorry
+-- ⟩
+
+
+set_option linter.unusedVariables false in
+/-- Source: [DM4Ever] figure 4 `loop_invar_sound`, as well as in `DelaySpecMonad.v` definitino `loop_invar`. -/
+theorem loop_invar (body : A -> ITree0 (A ⊕ B)) (a₀ : A)
+  (P : ITree0 B -> Prop) {P_eutt : RespEutt P}
+  (Inv : ITree0 (A ⊕ B) -> Prop) {Inv_eutt : RespEutt P}
+  (start : Inv (body a₀))
+  (step : ∀r, Inv r -> Inv (r >>= iter_lift body))
+  (stop : ∀t, Inv (t >>= fun b => return .inr b) -> P t)
+  : P (iter body a₀) ∨ Diverges (iter body a₀)
+  := trustITree "[DM4Ever] figure 4 `loop_invar_sound`, as well as in `DelaySpecMonad.v` definitino `loop_invar`"
