LeanBoogie/Woogie.lean
@@ -1,0 +1,146 @@
+import LeanBoogie.Boogie
+import LeanBoogie.Notation
+import LeanBoogie.ITree.ITree0W
+
+namespace LeanBoogie
+open ITree
+
+/-- This type doesn't support events on its `ITree`.
+  See section 4.5 in DM4Ever.
+
+  Reducing this type (with `S = BoogieState`), you get:
+  ```
+  S -> (ITree Empty (A × S) -> Prop) -> Prop
+  ```
+  Rearranging a little, you get the familiar predicate transformer type, from postc. to prec.:
+  ```
+  (ITree Empty (A × S) -> Prop) -> (S -> Prop)
+  ```
+  However, because `ITree0W` comes with some additional ballast such as monotonicity,
+  it is a little uglier still:
+  ```
+  (BoogieState →
+    (w : (p : ITree Empty (A × BoogieState) → Prop) -> RespEutt p → Prop) ×' Monotonic w)
+  ```
+-/
+def Woogie : Type -> Type := StateT BoogieState ITree0W
+
+example : Woogie A =
+  (BoogieState →
+    (w : (p : ITree Empty (A × BoogieState) → Prop) -> RespEutt p → Prop) ×' Monotonic w)
+  := by rfl
+
+def Woogie.mk
+  (w : BoogieState -> (post : ITree0 (A × BoogieState) → Prop) -> RespEutt post → Prop)
+  (w_mono : (s : BoogieState) -> Monotonic (w s))
+  : Woogie A
+  := fun s => ⟨w s, w_mono s⟩
+
+/-- Very unsafe version of `Woogie.mk`, which just uses `sorry` to solve monotonicity. -/
+def Woogie.mk!
+  (w : BoogieState -> (post : ITree0 (A × BoogieState) → Prop) → Prop)
+  : Woogie A
+  := fun s => ⟨fun post _hpost => w s post, sorry⟩
+
+def Woogie.pure (a : A) : Woogie A := fun s => return (a, s)
+def Woogie.bind (a : Woogie A) (b : A -> Woogie B) : Woogie B := fun s => a s >>= fun a => b a.fst a.snd
+
+instance : Monad Woogie where
+  pure := .pure
+  bind := .bind
+instance : LawfulMonad Woogie := sorry
+
+def Woogie.read (v : String) : Woogie Int :=
+  fun (s:BoogieState) => ⟨
+    fun (post) _ => post (.ret (s v, s)),
+    by unfold Monotonic; aesop
+  ⟩
+
+def Woogie.write (v : String) (a : Int) : Woogie Unit :=
+  fun s => ⟨
+    fun post _ => post (.ret ((), s.update v a)),
+    by rw [Monotonic]; aesop
+  ⟩
+
+/-- This is `θ_state` in DM4Ever. -/
+def Boogie.θ (b : Boogie Empty A) : Woogie A :=
+  fun s => ⟨
+    fun post _ => post (b s),
+    by rw [Monotonic]; aesop
+  ⟩
+
+instance : Theta (Boogie Empty) Woogie := ⟨Boogie.θ⟩
+
+/-- Specification ordering [DM4Aall 3.1]. -/
+def Woogie.le (w1 w2 : Woogie A) : Prop := ∀s p, (hp : RespEutt p) -> (w2 s).1 p hp -> (w1 s).1 p hp
+instance : LE (Woogie A) := ⟨Woogie.le⟩
+
+theorem Boogie.θ_pure : θ (return a) = (return a) := rfl
+theorem Boogie.θ_bind {a : Boogie Empty A} {b : A -> Boogie Empty B}
+  : θ (a >>= b) = (θ a >>= fun a => θ (b a))
+  := by
+    unfold θ
+    dsimp [Bind.bind, StateT.bind.eq_unfold]
+    unfold Woogie.bind
+    funext s
+    congr
+    funext post hpost
+    ext
+    simp_all only [Prod.exists]
+    constructor
+    . intro h
+      sorry
+    . intro h
+      cases h with
+      | inl h =>
+        have ⟨a1, s', converges, h2⟩ := h
+        sorry
+      | inr h_2 =>
+        sorry
+
+instance : LawfulTheta (Boogie Empty) (Woogie) := ⟨Boogie.θ_pure, Boogie.θ_bind⟩
+
+theorem Boogie.θ_read : θ (Boogie.read v) = (Woogie.read v) := by sorry
+theorem Boogie.θ_write : θ (Boogie.write v x) = (Woogie.write v x) := by sorry
+
+theorem Boogie.θ_ite [Decidable φ]
+  : θ (if φ then t else e)
+  = (if φ then θ t else θ e)
+  := by
+  split
+  next h => simp_all only
+  next h => simp_all only
+
+theorem Boogie.θ_ite' [Decidable φ]
+  : θ (if φ then t else e)
+  = Woogie.mk! (fun s post => (φ -> (θ t s).1 post sorry) ∧ (¬φ -> (θ e s).1 post sorry))
+  := by
+  split
+  next h => simp_all only [true_implies, not_true_eq_false, false_implies, and_true]; rfl
+  next h => simp_all only [false_implies, not_false_eq_true, true_implies, true_and]; rfl
+
+def BoogV {A : Type} (w : Woogie A) (b : Boogie Empty A) : Prop := θ b <= w
+
+theorem BoogV.ite [Decidable φ] {w : Woogie A}
+  (tru :  φ -> BoogV w t)
+  (fal : ¬φ -> BoogV w e)
+  : BoogV w (if φ then t else e)
+  := by aesop
+
+theorem BoogV.ite' [Decidable φ] {w : Woogie A} {t e : Boogie Empty A}
+  (tru :  φ -> θ t <= w)
+  (fal : ¬φ -> θ e <= w)
+  : θ (if φ then t else e) <= w
+  := by aesop
+
+theorem BoogV.ite'' [Decidable φ] {w : Woogie A}
+  (tru :  φ -> t <= w)
+  (fal : ¬φ -> e <= w)
+  : (if φ then t else e) <= w
+  := by aesop
+
+-- * Thoughts on interp vs θ
+-- `interp` is a monad morphism (from `ITree MemEv` to `StateT S (ITree Empty)` (aka Boogie))
+-- `θ` is a monad morphism (from `StateT S (ITree Empty)` to `StateT S (ITreeSpec Empty)` (aka Woogie))
+-- (1) ...so, you presumably can compose those two monad morphisms.
+-- (2) ...can you go the other way, first apply `θ` and then `interp`?
